.bot change for substitution inside eval

engine/PrisonersDilemma/Bots/TitForTatBot.lean
@@ -7,7 +7,7 @@ namespace PDNew.Bots
 -- Bot cooperates if the opponent cooperates against a cooperate probe. --
 def TitForTatBot : Prog :=
   .ite -- If then else
-    (.sim .opp (CooperateBot)) -- Simulate opponent against CooperateBot
+    (.sim .opp (.bot CooperateBot)) -- Simulate opponent against CooperateBot
     Action.C -- test action C
     (.const Action.C) -- if opponent cooperates, cooperate
     (.const Action.D) -- else, defect
