engine/PrisonersDilemma/Bots/EBot.lean
@@ -8,15 +8,15 @@ namespace PDNew.Bots
 
 def EBot : Prog :=
   .ite -- If then else
-    (.sim .opp DefectBot) -- Simulate opponent against DefectBot
+    (.sim .opp (.bot DefectBot)) -- Simulate opponent against DefectBot
     Action.C -- test action C
     (.const Action.D) -- if opponent cooperates, defect
     (.ite -- else, simulate opponent against CooperateBot
-      (.sim .opp CooperateBot)
+      (.sim .opp (.bot CooperateBot))
       Action.C -- test action C
       (.const Action.C) -- if opponent cooperates, cooperate
       (.ite -- else, simulate opponent against MirrorBot
-        (.sim .opp MirrorBot)
+        (.sim .opp (.bot MirrorBot))
         Action.C -- test action C
         (.const Action.C) -- if opponent cooperates, cooperate
         (.const Action.D))) -- else, defect
